ContextBasicDenotation/theories/BasicTypingFormula.v
@@ -77,11 +77,26 @@ with basic_tm_has_ltype : lty_env -> tm -> ty -> Prop :=
       basic_value_has_ltype Σ v1 (s1 →ₜ s2) ->
       basic_value_has_ltype Σ v2 s1 ->
       basic_tm_has_ltype Σ (tapp v1 v2) s2
-  | BTT_Match Σ v T et ef :
-      basic_value_has_ltype Σ v (TBase TBool) ->
-      basic_tm_has_ltype Σ et T ->
-      basic_tm_has_ltype Σ ef T ->
-      basic_tm_has_ltype Σ (tmatch v et ef) T.
+	  | BTT_Match Σ v T et ef :
+	      basic_value_has_ltype Σ v (TBase TBool) ->
+	      basic_tm_has_ltype Σ et T ->
+	      basic_tm_has_ltype Σ ef T ->
+	      basic_tm_has_ltype Σ (tmatch v et ef) T
+	  | BTT_TreeNode Σ root left right :
+	      basic_value_has_ltype Σ root (TBase TNat) ->
+	      basic_value_has_ltype Σ left (TBase TTree) ->
+	      basic_value_has_ltype Σ right (TBase TTree) ->
+	      basic_tm_has_ltype Σ (tnode root left right) (TBase TTree)
+	  | BTT_TreeMatch Σ v T eleaf enode (L : aset) :
+	      basic_value_has_ltype Σ v (TBase TTree) ->
+	      basic_tm_has_ltype Σ eleaf T ->
+	      (forall root left right,
+	        root ∉ L -> left ∉ L ∪ {[root]} ->
+	        right ∉ L ∪ {[root]} ∪ {[left]} ->
+	        basic_tm_has_ltype
+	          (tree_node_branch_open_env Σ root left right)
+	          (open_tree_node_branch root left right enode) T) ->
+	      basic_tm_has_ltype Σ (tmatchtree v eleaf enode) T.
 
 Scheme basic_value_has_ltype_ind' := Induction for basic_value_has_ltype Sort Prop
   with basic_tm_has_ltype_ind' := Induction for basic_tm_has_ltype Sort Prop.
@@ -98,11 +113,13 @@ Lemma basic_has_ltype_lvars_mutual :
     basic_tm_has_ltype Σ e T ->
     lvars_of_atoms (fv_tm e) ⊆ dom Σ).
 Proof.
-  apply basic_has_ltype_mutind; cbn [fv_value fv_tm]; intros; try set_solver.
+  apply basic_has_ltype_mutind; cbn [fv_value fv_tm]; intros.
+  - set_solver.
   - match goal with
     | Hlook : _ !! _ = Some _ |- _ =>
         apply elem_of_dom_2 in Hlook; set_solver
     end.
+  - set_solver.
   - set (y := fresh_for (L ∪ fv_tm e ∪ lvars_fv (dom Σ))).
     assert (Hy : y ∉ L ∪ fv_tm e ∪ lvars_fv (dom Σ)).
     { subst y. apply fresh_for_not_in. }
@@ -151,11 +168,12 @@ Proof.
       a ∈ lvars_fv (lvars_of_atoms (fv_value (open_value 0 (vfvar y) vf)))).
     { rewrite lvars_fv_of_atoms. apply Hopen. exact Ha. }
     pose proof (Hopened a HaOpen) as HaΣ.
-    apply elem_of_union in HaΣ as [HaΣ|HaΣ].
-    + apply elem_of_difference in HaΣ as [HaΣ _]. exact HaΣ.
-    + destruct (decide (0 ∈ lvars_bv (dom (typed_lty_env_bind Σ sx))));
-        set_solver.
-  - set (y := fresh_for (L ∪ fv_tm e2 ∪ lvars_fv (dom Σ))).
+	    apply elem_of_union in HaΣ as [HaΣ|HaΣ].
+	    + apply elem_of_difference in HaΣ as [HaΣ _]. exact HaΣ.
+	    + destruct (decide (0 ∈ lvars_bv (dom (typed_lty_env_bind Σ sx))));
+	        set_solver.
+  - set_solver.
+	  - set (y := fresh_for (L ∪ fv_tm e2 ∪ lvars_fv (dom Σ))).
     assert (Hy : y ∉ L ∪ fv_tm e2 ∪ lvars_fv (dom Σ)).
     { subst y. apply fresh_for_not_in. }
     match goal with
@@ -182,11 +200,136 @@ Proof.
       assert (HaOpen :
         a ∈ lvars_fv (lvars_of_atoms (fv_tm (open_tm 0 (vfvar y) e2)))).
       { rewrite lvars_fv_of_atoms. apply Hopen. exact Ha. }
-      pose proof (Hopened a HaOpen) as HaΣ.
-      apply elem_of_union in HaΣ as [HaΣ|HaΣ].
-      * apply elem_of_difference in HaΣ as [HaΣ _]. exact HaΣ.
-      * destruct (decide (0 ∈ lvars_bv (dom (typed_lty_env_bind Σ T1))));
-          set_solver.
+	      pose proof (Hopened a HaOpen) as HaΣ.
+		      apply elem_of_union in HaΣ as [HaΣ|HaΣ].
+		      * apply elem_of_difference in HaΣ as [HaΣ _]. exact HaΣ.
+		      * destruct (decide (0 ∈ lvars_bv (dom (typed_lty_env_bind Σ T1))));
+		          set_solver.
+  - set_solver.
+  - set_solver.
+  - set_solver.
+  - set_solver.
+		  - set (root := fresh_for
+	      (L ∪ fv_tm enode ∪ lvars_fv (dom Σ))).
+	    assert (Hroot : root ∉ L ∪ fv_tm enode ∪ lvars_fv (dom Σ)).
+	    { subst root. apply fresh_for_not_in. }
+	    set (left0 := fresh_for
+	      (L ∪ fv_tm enode ∪ lvars_fv (dom Σ) ∪ {[root]})).
+	    assert (Hleft : left0 ∉
+	      L ∪ fv_tm enode ∪ lvars_fv (dom Σ) ∪ {[root]}).
+	    { subst left0. apply fresh_for_not_in. }
+	    set (right0 := fresh_for
+	      (L ∪ fv_tm enode ∪ lvars_fv (dom Σ) ∪ {[root]} ∪ {[left0]})).
+		    assert (Hright : right0 ∉
+		      L ∪ fv_tm enode ∪ lvars_fv (dom Σ) ∪ {[root]} ∪ {[left0]}).
+		    { subst right0. apply fresh_for_not_in. }
+		    assert (HrootL : root ∉ L).
+		    {
+		      intros Hin. apply Hroot.
+		      apply elem_of_union_l. apply elem_of_union_l. exact Hin.
+		    }
+		    assert (HleftL : left0 ∉ L).
+		    {
+		      intros Hin. apply Hleft.
+		      apply elem_of_union_l. apply elem_of_union_l.
+		      apply elem_of_union_l. exact Hin.
+		    }
+			    assert (HrightL : right0 ∉ L).
+			    {
+			      intros Hin. apply Hright.
+			      apply elem_of_union_l. apply elem_of_union_l.
+			      apply elem_of_union_l. apply elem_of_union_l. exact Hin.
+			    }
+				    assert (Hleft_nested : left0 ∉ L ∪ {[root]}).
+				    {
+				      intros Hin. apply Hleft.
+				      apply elem_of_union in Hin as [Hin|Hin].
+				      - apply elem_of_union_l. apply elem_of_union_l.
+				        apply elem_of_union_l. exact Hin.
+				      - apply elem_of_union_r. exact Hin.
+				    }
+				    assert (Hright_nested : right0 ∉ L ∪ {[root]} ∪ {[left0]}).
+				    {
+				      intros Hin. apply Hright.
+				      apply elem_of_union in Hin as [Hin|Hin].
+				      - apply elem_of_union in Hin as [Hin|Hin].
+				        + apply elem_of_union_l. apply elem_of_union_l.
+				          apply elem_of_union_l. apply elem_of_union_l. exact Hin.
+				        + apply elem_of_union_l. apply elem_of_union_r. exact Hin.
+				      - apply elem_of_union_r. exact Hin.
+				    }
+			    match goal with
+			    | Hopen_typed : forall root left right,
+			        root ∉ _ -> left ∉ _ ∪ {[root]} ->
+			        right ∉ _ ∪ {[root]} ∪ {[left]} ->
+			        lvars_of_atoms (fv_tm _) ⊆ _ |- _ =>
+			        pose proof (Hopen_typed root left0 right0
+			          HrootL Hleft_nested Hright_nested) as Hopened
+				    end.
+		    apply lvars_fv_mono in Hopened.
+		    intros u Hu.
+		    unfold lvars_of_atoms in Hu.
+		    apply elem_of_map in Hu as [a [-> Ha]].
+	    apply elem_of_union in Ha as [Ha|Ha].
+	    + apply elem_of_union in Ha as [Ha|Ha].
+	      * match goal with
+	        | IH : lvars_of_atoms (fv_value _) ⊆ dom Σ |- _ => apply IH
+	        end.
+	        unfold lvars_of_atoms. apply elem_of_map.
+	        exists a. split; [reflexivity|exact Ha].
+	      * match goal with
+	        | IH : lvars_of_atoms (fv_tm _) ⊆ dom Σ |- _ => apply IH
+	        end.
+	        unfold lvars_of_atoms. apply elem_of_map.
+	        exists a. split; [reflexivity|exact Ha].
+	    + apply lvars_fv_elem.
+		        assert (HaOpen : a ∈ fv_tm
+		          (open_tree_node_branch root left0 right0 enode)).
+		        {
+		          unfold open_tree_node_branch, open_tree_node_branch_value.
+		          apply (open_fv_tm'
+		            (open_tm 1 (vfvar left0)
+		              (open_tm 0 (vfvar root) enode)) (vfvar right0) 2).
+		          apply (open_fv_tm'
+		            (open_tm 0 (vfvar root) enode) (vfvar left0) 1).
+		          apply (open_fv_tm' enode (vfvar root) 0).
+		          exact Ha.
+		        }
+	        assert (HaOpenLvars :
+	          a ∈ lvars_fv
+	            (lvars_of_atoms
+	              (fv_tm (open_tree_node_branch root left0 right0 enode)))).
+		        { rewrite lvars_fv_of_atoms. exact HaOpen. }
+		        pose proof (Hopened a HaOpenLvars) as HaBranchΣ.
+		        pose proof (tree_node_branch_open_env_lvars_fv_dom_subset
+		          Σ root left0 right0 a HaBranchΣ) as HaΣ.
+		        assert (HrootFV : root ∉ fv_tm enode).
+		        {
+		          intros Hin. apply Hroot.
+		          apply elem_of_union_l. apply elem_of_union_r. exact Hin.
+		        }
+		        assert (HleftFV : left0 ∉ fv_tm enode).
+		        {
+		          intros Hin. apply Hleft.
+		          apply elem_of_union_l. apply elem_of_union_l.
+		          apply elem_of_union_r. exact Hin.
+		        }
+		        assert (HrightFV : right0 ∉ fv_tm enode).
+		        {
+		          intros Hin. apply Hright.
+		          apply elem_of_union_l. apply elem_of_union_l.
+		          apply elem_of_union_l. apply elem_of_union_r. exact Hin.
+		        }
+		        apply elem_of_union in HaΣ as [HaΣ|HaRight].
+		        * apply elem_of_union in HaΣ as [HaΣ|HaLeft].
+		          -- apply elem_of_union in HaΣ as [HaBase|HaRoot].
+		             ++ exact HaBase.
+		             ++ rewrite elem_of_singleton in HaRoot.
+		                subst a. contradiction.
+		          -- rewrite elem_of_singleton in HaLeft.
+		             subst a. contradiction.
+		        * rewrite elem_of_singleton in HaRight.
+		          subst a. contradiction.
 Qed.
 
 Lemma basic_value_has_ltype_lvars Σ v T :
@@ -253,6 +396,19 @@ Proof.
   apply typed_lty_env_bind_mono. exact Hsub.
 Qed.
 
+Lemma tree_node_branch_open_env_mono
+    (Σ Σ' : lty_env) root left right :
+  Σ ⊆ Σ' ->
+  tree_node_branch_open_env Σ root left right ⊆
+  tree_node_branch_open_env Σ' root left right.
+Proof.
+  intros Hsub.
+  unfold tree_node_branch_open_env, tree_node_branch_bound_env.
+  repeat apply lty_env_open_one_mono.
+  repeat apply typed_lty_env_bind_mono.
+  exact Hsub.
+Qed.
+
 Lemma basic_has_ltype_weaken_mutual :
   (forall Σ v T,
     basic_value_has_ltype Σ v T ->
@@ -278,6 +434,12 @@ Proof.
     + eapply H; exact H1.
     + intros x Hx. eapply H0; [exact Hx|].
       apply lty_env_open_one_typed_bind_mono. exact H1.
+	  - eapply BTT_TreeMatch with (L := L).
+	    + eapply H; exact H2.
+	    + eapply H0; exact H2.
+	    + intros root left right Hroot Hleft Hright.
+	      eapply H1; [exact Hroot|exact Hleft|exact Hright|].
+	      apply tree_node_branch_open_env_mono. exact H2.
 Qed.
 
 Lemma basic_value_has_ltype_weaken Σ Σ' v T :
@@ -351,19 +513,80 @@ Proof.
       apply elem_of_union in Hv as [Hv|Hv].
       * rewrite elem_of_singleton in Hv. subst v. exact I.
       * exact (H0 v Hv).
-  - eapply LC_lete with (L := L ∪ lvars_fv (dom Σ)).
-    + eauto.
-    + intros x Hx. eapply H0; [set_solver|].
-      * intros v Hv.
+	  - eapply LC_lete with (L := L ∪ lvars_fv (dom Σ)).
+	    + eauto.
+	    + intros x Hx. eapply H0; [set_solver|].
+	      * intros v Hv.
         assert (Hfreshx : LVFree x ∉ dom Σ).
         { intros Hdom.
           apply Hx. apply elem_of_union_r. apply lvars_fv_elem. exact Hdom. }
         pose proof (typed_lty_env_bind_open_current x Σ T1 Hfreshx H1) as Henv.
         rewrite Henv in Hv.
-        rewrite dom_insert in Hv.
-        apply elem_of_union in Hv as [Hv|Hv].
-        -- rewrite elem_of_singleton in Hv. subst v. exact I.
-        -- exact (H1 v Hv).
+	        rewrite dom_insert in Hv.
+	        apply elem_of_union in Hv as [Hv|Hv].
+	        -- rewrite elem_of_singleton in Hv. subst v. exact I.
+	        -- exact (H1 v Hv).
+		  - eapply LC_matchtree with (L := L ∪ lvars_fv (dom Σ)).
+		    + eauto.
+		    + eauto.
+		    + intros root left right Hroot Hleft Hright.
+		      assert (HrootL : root ∉ L).
+		      { intros Hin. apply Hroot. apply elem_of_union_l. exact Hin. }
+		      assert (HleftL : left ∉ L ∪ {[root]}).
+		      {
+		        intros Hin. apply Hleft.
+		        apply elem_of_union in Hin as [Hin|Hin];
+		          [apply elem_of_union_l; apply elem_of_union_l; exact Hin
+		          |apply elem_of_union_r; exact Hin].
+		      }
+		      assert (HrightL : right ∉ L ∪ {[root]} ∪ {[left]}).
+		      {
+		        intros Hin. apply Hright.
+		        apply elem_of_union in Hin as [Hin|Hin].
+		        { apply elem_of_union in Hin as [Hin|Hin].
+		          { apply elem_of_union_l. apply elem_of_union_l.
+		            apply elem_of_union_l. exact Hin. }
+		          { apply elem_of_union_l. apply elem_of_union_r. exact Hin. } }
+		        { apply elem_of_union_r. exact Hin. }
+		      }
+		      assert (HrootΣ : root ∉ lvars_fv (dom Σ)).
+		      { intros Hin. apply Hroot. apply elem_of_union_r. exact Hin. }
+		      assert (HleftΣ : left ∉ lvars_fv (dom Σ)).
+		      {
+		        intros Hin. apply Hleft.
+		        apply elem_of_union_l. apply elem_of_union_r. exact Hin.
+		      }
+		      assert (HrightΣ : right ∉ lvars_fv (dom Σ)).
+		      {
+		        intros Hin. apply Hright.
+		        apply elem_of_union_l. apply elem_of_union_l.
+		        apply elem_of_union_r. exact Hin.
+		      }
+			      assert (Hroot_left : root <> left).
+			      {
+			        intro Heq. apply Hleft. apply elem_of_union_r.
+			        rewrite elem_of_singleton. symmetry. exact Heq.
+			      }
+			      assert (Hroot_right : root <> right).
+			      {
+			        intro Heq. apply Hright. apply elem_of_union_l.
+			        apply elem_of_union_r.
+			        rewrite elem_of_singleton. symmetry. exact Heq.
+			      }
+			      assert (Hleft_right : left <> right).
+			      {
+			        intro Heq. apply Hright. apply elem_of_union_r.
+			        rewrite elem_of_singleton. symmetry. exact Heq.
+			      }
+		      eapply H1; [exact HrootL|exact HleftL|exact HrightL|].
+		      apply tree_node_branch_open_env_lc_dom.
+		      * exact H2.
+		      * exact HrootΣ.
+		      * exact HleftΣ.
+		      * exact HrightΣ.
+		      * exact Hroot_left.
+		      * exact Hroot_right.
+		      * exact Hleft_right.
 Qed.
 
 Lemma basic_value_has_ltype_lc Σ v T :
@@ -388,8 +611,11 @@ Lemma basic_tm_has_ltype_ret_fvar_lookup
   Σ !! LVFree x = Some T.
 Proof.
   intros Hty.
-  inversion Hty as [Γ v U Hval| | | |]; subst; clear Hty.
-  inversion Hval; subst; eauto.
+  inversion Hty; subst; clear Hty.
+  match goal with
+  | H : basic_value_has_ltype _ (vfvar x) _ |- _ =>
+      inversion H; subst; eauto
+  end.
 Qed.
 
 Lemma lty_env_open_one_typed_bind_lookup_free_ne
@@ -451,7 +677,7 @@ Proof.
   destruct v as [k|z].
   - exfalso.
     assert (k ∈ lvars_bv Dbody) by (rewrite lvars_bv_elem; exact HvD).
-    rewrite Hbv in H. set_solver.
+    rewrite Hbv in H. clear -H. set_solver.
   - destruct (decide (z = x)) as [->|Hzx].
     + rewrite lty_env_open_one_typed_bind_lookup_current.
       rewrite lty_env_open_one_typed_bind_lookup_current in Hlook.
@@ -467,6 +693,159 @@ Proof.
         contradiction.
       }
       exact HzD.
+Qed.
+
+Lemma lty_env_restrict_tree_branch_body_subset
+    (Σ : lty_env) root left right Dbody D :
+  root ∉ lvars_fv D ->
+  left ∉ lvars_fv D ->
+  right ∉ lvars_fv D ->
+  lvars_bv Dbody = ∅ ->
+  Dbody ⊆ D ∪ {[LVFree root]} ∪ {[LVFree left]} ∪ {[LVFree right]} ->
+  storeA_restrict
+    (<[LVFree right := TBase TTree]>
+      (<[LVFree left := TBase TTree]>
+        (<[LVFree root := TBase TNat]> Σ))) Dbody ⊆
+  <[LVFree right := TBase TTree]>
+    (<[LVFree left := TBase TTree]>
+      (<[LVFree root := TBase TNat]> (storeA_restrict Σ D))).
+Proof.
+  intros HrootD HleftD HrightD Hbv Hsub.
+  apply map_subseteq_spec. intros v U Hlook.
+  apply storeA_restrict_lookup_some in Hlook as [HvD Hlook].
+  destruct v as [k|z].
+  - exfalso.
+    assert (k ∈ lvars_bv Dbody) by (rewrite lvars_bv_elem; exact HvD).
+    rewrite Hbv in H. clear -H. set_solver.
+	  - destruct (decide (z = right)) as [->|Hzr].
+	    + rewrite lookup_insert in Hlook.
+	      destruct (decide (LVFree right = LVFree right)) as [_|Hbad] in Hlook;
+	        [|congruence].
+	      rewrite lookup_insert.
+	      destruct (decide (LVFree right = LVFree right)) as [_|Hbad];
+	        [exact Hlook|congruence].
+	    + rewrite lookup_insert_ne in Hlook by (intros Heq; inversion Heq; congruence).
+	      rewrite lookup_insert_ne by (intros Heq; inversion Heq; congruence).
+	      destruct (decide (z = left)) as [->|Hzl].
+	      * rewrite lookup_insert in Hlook.
+	        destruct (decide (LVFree left = LVFree left)) as [_|Hbad] in Hlook;
+	          [|congruence].
+	        rewrite lookup_insert.
+	        destruct (decide (LVFree left = LVFree left)) as [_|Hbad];
+	          [exact Hlook|congruence].
+	      * rewrite lookup_insert_ne in Hlook by (intros Heq; inversion Heq; congruence).
+	        rewrite lookup_insert_ne by (intros Heq; inversion Heq; congruence).
+	        destruct (decide (z = root)) as [->|Hzroot].
+	        -- rewrite lookup_insert in Hlook.
+	           destruct (decide (LVFree root = LVFree root)) as [_|Hbad] in Hlook;
+	             [|congruence].
+	           rewrite lookup_insert.
+	           destruct (decide (LVFree root = LVFree root)) as [_|Hbad];
+	             [exact Hlook|congruence].
+	        -- rewrite lookup_insert_ne in Hlook by (intros Heq; inversion Heq; congruence).
+	           rewrite lookup_insert_ne by (intros Heq; inversion Heq; congruence).
+	           apply (storeA_restrict_lookup_some_2 _ _ _ _ Hlook).
+		   assert (LVFree z ∈ D).
+		   {
+			     specialize (Hsub _ HvD).
+			     set_unfold in Hsub.
+			     set_unfold.
+		     intuition; try congruence;
+		       try match goal with
+		       | H : LVFree _ = LVFree _ |- _ => inversion H; congruence
+		       end.
+		   }
+		   exact H.
+Qed.
+
+Lemma lty_env_restrict_tree_node_branch_open_env_body_subset
+    (Σ : lty_env) root left right Dbody D :
+  root <> left ->
+  root <> right ->
+  left <> right ->
+  root ∉ lvars_fv D ->
+  left ∉ lvars_fv D ->
+  right ∉ lvars_fv D ->
+  lvars_bv Dbody = ∅ ->
+  Dbody ⊆ D ∪ {[LVFree root]} ∪ {[LVFree left]} ∪ {[LVFree right]} ->
+  storeA_restrict (tree_node_branch_open_env Σ root left right) Dbody ⊆
+  tree_node_branch_open_env (storeA_restrict Σ D) root left right.
+Proof.
+  intros Hroot_left Hroot_right Hleft_right HrootD HleftD HrightD Hbv Hsub.
+  apply map_subseteq_spec. intros v U Hlook.
+  apply storeA_restrict_lookup_some in Hlook as [HvD Hlook].
+  destruct v as [k|z].
+  - exfalso.
+    assert (k ∈ lvars_bv Dbody) by (rewrite lvars_bv_elem; exact HvD).
+    rewrite Hbv in H. clear -H. set_solver.
+  - replace (tree_node_branch_open_env Σ root left right !! LVFree z)
+      with ((<[LVFree right := TBase TTree]>
+        (<[LVFree left := TBase TTree]>
+          (<[LVFree root := TBase TNat]> Σ))) !! LVFree z) in Hlook.
+    2:{ symmetry. apply tree_node_branch_open_env_lookup_free; assumption. }
+    replace (tree_node_branch_open_env (storeA_restrict Σ D) root left right
+        !! LVFree z)
+      with ((<[LVFree right := TBase TTree]>
+        (<[LVFree left := TBase TTree]>
+          (<[LVFree root := TBase TNat]> (storeA_restrict Σ D)))) !! LVFree z).
+    2:{ symmetry. apply tree_node_branch_open_env_lookup_free; assumption. }
+    destruct (decide (z = right)) as [->|Hzr].
+    + rewrite lookup_insert in Hlook.
+      destruct (decide (LVFree right = LVFree right)) as [_|Hbad] in Hlook;
+        [|congruence].
+      rewrite lookup_insert.
+      destruct (decide (LVFree right = LVFree right)) as [_|Hbad];
+        [exact Hlook|congruence].
+    + rewrite lookup_insert_ne in Hlook by (intros Heq; inversion Heq; congruence).
+      rewrite lookup_insert_ne by (intros Heq; inversion Heq; congruence).
+      destruct (decide (z = left)) as [->|Hzl].
+      * rewrite lookup_insert in Hlook.
+        destruct (decide (LVFree left = LVFree left)) as [_|Hbad] in Hlook;
+          [|congruence].
+        rewrite lookup_insert.
+        destruct (decide (LVFree left = LVFree left)) as [_|Hbad];
+          [exact Hlook|congruence].
+      * rewrite lookup_insert_ne in Hlook by (intros Heq; inversion Heq; congruence).
+        rewrite lookup_insert_ne by (intros Heq; inversion Heq; congruence).
+        destruct (decide (z = root)) as [->|Hzroot].
+        -- rewrite lookup_insert in Hlook.
+           destruct (decide (LVFree root = LVFree root)) as [_|Hbad] in Hlook;
+             [|congruence].
+           rewrite lookup_insert.
+           destruct (decide (LVFree root = LVFree root)) as [_|Hbad];
+             [exact Hlook|congruence].
+        -- rewrite lookup_insert_ne in Hlook by (intros Heq; inversion Heq; congruence).
+           rewrite lookup_insert_ne by (intros Heq; inversion Heq; congruence).
+           apply (storeA_restrict_lookup_some_2 _ _ _ _ Hlook).
+           assert (HzD : LVFree z ∈ D).
+           {
+             specialize (Hsub _ HvD).
+             apply elem_of_union in Hsub as [Hsub|Hright].
+             - apply elem_of_union in Hsub as [Hsub|Hleft].
+               + apply elem_of_union in Hsub as [HzD|Hroot]; [exact HzD|].
+                 rewrite elem_of_singleton in Hroot. inversion Hroot. subst z.
+                 contradiction.
+               + rewrite elem_of_singleton in Hleft. inversion Hleft. subst z.
+                 contradiction.
+             - rewrite elem_of_singleton in Hright. inversion Hright. subst z.
+               contradiction.
+           }
+           exact HzD.
+Qed.
+
+Lemma lc_matchtree_iff_parts v eleaf enode :
+  lc_tm (tmatchtree v eleaf enode) ->
+  lc_value v /\
+  lc_tm eleaf /\
+	  exists L : aset,
+	    forall root left right,
+	      root ∉ L ->
+	      left ∉ L ∪ {[root]} ->
+	      right ∉ L ∪ {[root]} ∪ {[left]} ->
+	      lc_tm (open_tree_node_branch root left right enode).
+Proof.
+  intros Hlc. inversion Hlc; subst.
+  repeat split; eauto.
 Qed.
 
 Lemma basic_has_ltype_restrict_lvars_lc_mutual :
@@ -601,6 +980,184 @@ Proof.
       | Hsub : tm_lvars (tmatch _ _ _) ⊆ _ |- _ =>
           cbn [tm_lvars tm_lvars_at] in Hsub; set_solver
       end.
+  - match goal with
+    | Hlc : lc_tm (tnode _ _ _) |- _ =>
+        inversion Hlc; subst; clear Hlc
+    end.
+    eapply BTT_TreeNode.
+    + eapply H; eauto.
+      match goal with
+      | Hsub : tm_lvars (tnode _ _ _) ⊆ _ |- _ =>
+          cbn [tm_lvars tm_lvars_at] in Hsub; set_solver
+      end.
+    + eapply H0; eauto.
+      match goal with
+      | Hsub : tm_lvars (tnode _ _ _) ⊆ _ |- _ =>
+          cbn [tm_lvars tm_lvars_at] in Hsub; set_solver
+      end.
+    + eapply H1; eauto.
+      match goal with
+      | Hsub : tm_lvars (tnode _ _ _) ⊆ _ |- _ =>
+          cbn [tm_lvars tm_lvars_at] in Hsub; set_solver
+      end.
+  - match goal with
+    | Hlc : lc_tm (tmatchtree _ _ _) |- _ =>
+        apply lc_matchtree_iff_parts in Hlc as [Hlcv [Hlcleaf [Llc Hlcnode]]]
+    end.
+		    eapply BTT_TreeMatch with
+		      (L := L ∪ Llc ∪ lvars_fv D ∪ lvars_fv (dom Σ) ∪ fv_tm enode).
+		    + assert (Hv_sub : value_lvars v ⊆ D).
+		      {
+		        intros u Hu. apply H3.
+		        cbn [tm_lvars tm_lvars_at].
+		        apply elem_of_union_l. apply elem_of_union_l. exact Hu.
+		      }
+		      eapply H; [exact Hlcv|exact Hv_sub].
+		    + assert (Hleaf_sub : tm_lvars eleaf ⊆ D).
+		      {
+		        intros u Hu. apply H3.
+		        cbn [tm_lvars tm_lvars_at].
+		        apply elem_of_union_l. apply elem_of_union_r. exact Hu.
+		      }
+		      eapply H0; [exact Hlcleaf|exact Hleaf_sub].
+		    + intros root left right Hroot Hleft Hright.
+		      assert (HrootL : root ∉ L).
+		      {
+		        intros Hin. apply Hroot.
+		        repeat apply elem_of_union_l. exact Hin.
+		      }
+		      assert (HleftL : left ∉ L ∪ {[root]}).
+		      {
+		        intros Hin. apply Hleft.
+		        apply elem_of_union in Hin as [Hin|Hin].
+		        - apply elem_of_union_l. repeat apply elem_of_union_l. exact Hin.
+		        - apply elem_of_union_r. exact Hin.
+		      }
+		      assert (HrightL : right ∉ L ∪ {[root]} ∪ {[left]}).
+		      {
+		        intros Hin. apply Hright.
+		        apply elem_of_union in Hin as [Hin|Hin].
+		        - apply elem_of_union in Hin as [Hin|Hin].
+		          + apply elem_of_union_l. apply elem_of_union_l.
+		            repeat apply elem_of_union_l. exact Hin.
+		          + apply elem_of_union_l. apply elem_of_union_r. exact Hin.
+		        - apply elem_of_union_r. exact Hin.
+		      }
+		      assert (HrootD : root ∉ lvars_fv D).
+		      {
+		        intros Hin. apply Hroot.
+		        apply elem_of_union_l. apply elem_of_union_l.
+		        apply elem_of_union_r. exact Hin.
+		      }
+		      assert (HleftD : left ∉ lvars_fv D).
+		      {
+		        intros Hin. apply Hleft.
+		        apply elem_of_union_l. apply elem_of_union_l.
+		        apply elem_of_union_l. apply elem_of_union_r. exact Hin.
+		      }
+		      assert (HrightD : right ∉ lvars_fv D).
+		      {
+		        intros Hin. apply Hright.
+		        apply elem_of_union_l. apply elem_of_union_l.
+		        apply elem_of_union_l. apply elem_of_union_l.
+		        apply elem_of_union_r. exact Hin.
+		      }
+		      assert (HrootΣ : root ∉ lvars_fv (dom Σ)).
+		      {
+		        intros Hin. apply Hroot.
+		        apply elem_of_union_l. apply elem_of_union_r. exact Hin.
+		      }
+		      assert (HleftΣ : left ∉ lvars_fv (dom Σ)).
+		      {
+		        intros Hin. apply Hleft.
+		        apply elem_of_union_l. apply elem_of_union_l.
+		        apply elem_of_union_r. exact Hin.
+		      }
+		      assert (HrightΣ : right ∉ lvars_fv (dom Σ)).
+		      {
+		        intros Hin. apply Hright.
+		        apply elem_of_union_l. apply elem_of_union_l.
+		        apply elem_of_union_l. apply elem_of_union_r. exact Hin.
+		      }
+		      assert (Hroot_left : root <> left).
+		      {
+		        intro Heq. apply Hleft. apply elem_of_union_r.
+		        rewrite elem_of_singleton. symmetry. exact Heq.
+		      }
+		      assert (Hroot_right : root <> right).
+		      {
+		        intro Heq. apply Hright. apply elem_of_union_l.
+		        apply elem_of_union_r.
+		        rewrite elem_of_singleton. symmetry. exact Heq.
+		      }
+			      assert (Hleft_right : left <> right).
+			      {
+			        intro Heq. apply Hright. apply elem_of_union_r.
+			        rewrite elem_of_singleton. symmetry. exact Heq.
+			      }
+			      assert (HrootLlc : root ∉ Llc) by (clear -Hroot; set_solver).
+			      assert (HleftLlc : left ∉ Llc ∪ {[root]})
+			        by (clear -Hleft; set_solver).
+			      assert (HrightLlc : right ∉ Llc ∪ {[root]} ∪ {[left]})
+			        by (clear -Hright; set_solver).
+			      assert (Hbranch_lc :
+			        lc_tm (open_tree_node_branch root left right enode)).
+			      { eapply Hlcnode; [exact HrootLlc|exact HleftLlc|exact HrightLlc]. }
+		      pose proof (H1 root left right HrootL HleftL HrightL) as IHbranch.
+		      eapply basic_tm_has_ltype_weaken.
+		      * apply IHbranch.
+		        -- exact Hbranch_lc.
+	        -- reflexivity.
+			      * eapply lty_env_restrict_tree_node_branch_open_env_body_subset.
+			        -- exact Hroot_left.
+			        -- exact Hroot_right.
+			        -- exact Hleft_right.
+			        -- exact HrootD.
+			        -- exact HleftD.
+			        -- exact HrightD.
+			        -- apply tm_lvars_no_bv_of_lc.
+			           exact Hbranch_lc.
+	        -- intros u Hu.
+	           rewrite (tm_lvars_lc_eq_atoms
+	             (open_tree_node_branch root left right enode)) in Hu.
+	           2:{ exact Hbranch_lc. }
+           unfold lvars_of_atoms in Hu.
+           apply elem_of_map in Hu as [a [-> Ha0]].
+           unfold open_tree_node_branch, open_tree_node_branch_value in Ha0.
+	           pose proof (open_fv_tm
+	             (open_tm 1 (vfvar left) (open_tm 0 (vfvar root) enode))
+	             (vfvar right) 2 a Ha0) as Ha1.
+	           cbn [fv_value] in Ha1.
+	           apply elem_of_union in Ha1 as [Ha1|Ha1].
+	           ++ rewrite elem_of_singleton in Ha1. subst a.
+	              apply elem_of_union_r. apply elem_of_singleton. reflexivity.
+	           ++ pose proof (open_fv_tm
+	                (open_tm 0 (vfvar root) enode) (vfvar left) 1 a Ha1) as Ha2.
+	              cbn [fv_value] in Ha2.
+	              apply elem_of_union in Ha2 as [Ha2|Ha2].
+	              ** rewrite elem_of_singleton in Ha2. subst a.
+	                 apply elem_of_union_l. apply elem_of_union_r.
+	                 apply elem_of_singleton. reflexivity.
+	              ** pose proof (open_fv_tm enode (vfvar root) 0 a Ha2) as Ha3.
+	                 cbn [fv_value] in Ha3.
+	                 apply elem_of_union in Ha3 as [Ha3|Ha3].
+	                 --- rewrite elem_of_singleton in Ha3. subst a.
+	                     apply elem_of_union_l. apply elem_of_union_l.
+	                     apply elem_of_union_r. apply elem_of_singleton.
+	                     reflexivity.
+                 --- assert (LVFree a ∈ D) as HaD.
+                     {
+                       match goal with
+                       | Hsub : tm_lvars (tmatchtree _ _ _) ⊆ D |- _ =>
+                           cbn [tm_lvars tm_lvars_at] in Hsub;
+                           apply Hsub
+                       end.
+                       apply elem_of_union_r.
+                       apply lvars_fv_elem.
+	                       rewrite tm_lvars_at_fv. exact Ha3.
+	                     }
+	                     apply elem_of_union_l. apply elem_of_union_l.
+	                     apply elem_of_union_l. exact HaD.
 Qed.
 
 Lemma basic_value_has_ltype_restrict_lvars_lc Σ v T D :
@@ -695,6 +1252,24 @@ Proof.
     pose proof (H0 x ltac:(set_solver)) as Hbody.
     rewrite lvar_store_open_bind_atom_store by set_solver.
     exact Hbody.
+  - match goal with
+    | |- basic_tm_has_ltype (atom_env_to_lty_env ?Γ) _ _ =>
+        eapply BTT_TreeMatch with (L := L ∪ dom Γ)
+    end; eauto.
+    intros root left right Hroot Hleft Hright.
+	    pose proof (H1 root left right
+	      ltac:(set_solver) ltac:(set_solver) ltac:(set_solver)) as Hbody.
+	    rewrite (tree_node_branch_open_env_norm
+	      (atom_env_to_lty_env Γ) root left right).
+	    2:{ apply atom_store_to_lvar_store_closed. }
+	    2:{ rewrite atom_store_to_lvar_store_dom. clear -Hroot. set_solver. }
+	    2:{ rewrite atom_store_to_lvar_store_dom. clear -Hleft. set_solver. }
+	    2:{ rewrite atom_store_to_lvar_store_dom. clear -Hright. set_solver. }
+	    2:{ clear -Hleft. set_solver. }
+	    2:{ clear -Hright. set_solver. }
+	    2:{ clear -Hright. set_solver. }
+	    rewrite <- !atom_store_to_lvar_store_insert.
+	    exact Hbody.
 Qed.
 
 Lemma basic_value_has_ltype_of_atom_env_typing Δ v T :
@@ -751,6 +1326,28 @@ Proof.
   - eapply TT_Op; eauto.
   - eapply TT_App; eauto.
   - eapply TT_Match; eauto.
+  - eapply TT_TreeNode; eauto.
+  - eapply TT_TreeMatch with (L := L ∪ dom Δ).
+    + eauto.
+    + eauto.
+    + intros root left right Hroot Hleft Hright.
+      specialize (H1 root left right
+        ltac:(set_solver) ltac:(set_solver) ltac:(set_solver)
+        (<[right := TBase TTree]>
+          (<[left := TBase TTree]>
+            (<[root := TBase TNat]> Δ)))).
+		      apply H1.
+		      rewrite (tree_node_branch_open_env_norm
+		        (atom_env_to_lty_env Δ) root left right).
+		      2:{ apply atom_store_to_lvar_store_closed. }
+		      2:{ rewrite atom_store_to_lvar_store_dom. clear -Hroot. set_solver. }
+		      2:{ rewrite atom_store_to_lvar_store_dom. clear -Hleft. set_solver. }
+		      2:{ rewrite atom_store_to_lvar_store_dom. clear -Hright. set_solver. }
+		      2:{ clear -Hleft. set_solver. }
+		      2:{ clear -Hright. set_solver. }
+		      2:{ clear -Hright. set_solver. }
+		      rewrite <- !atom_store_to_lvar_store_insert.
+		      reflexivity.
 Qed.
 
 Lemma basic_tm_has_ltype_to_atom_env_typing Δ e T :
@@ -888,6 +1485,12 @@ Proof.
     | IH : forall T2, basic_tm_has_ltype _ _ T2 -> _,
       Hthen : basic_tm_has_ltype _ _ _ |- _ =>
         exact (IH _ Hthen)
+    end.
+  - reflexivity.
+  - match goal with
+    | IH : forall T2, basic_tm_has_ltype _ _ T2 -> _,
+      Hleaf : basic_tm_has_ltype _ _ _ |- _ =>
+        exact (IH _ Hleaf)
     end.
 Qed.
 
